Fix tests

test/Grammars/Test/DemoContextSensitive.lean
@@ -13,18 +13,20 @@ This file contains example context-sensitive grammars and sample derivation proo
 -/
 
 inductive Te
-| a_ : Te
-| b_ : Te
-| c_ : Te
+  | a_ : Te
+  | b_ : Te
+  | c_ : Te
+  deriving DecidableEq
 
 inductive Nt
-| B_ : Nt
-| C_ : Nt
-| R_ : Nt
-| S_ : Nt
-| X_ : Nt
-| Y_ : Nt
-| Z_ : Nt
+  | B_ : Nt
+  | C_ : Nt
+  | R_ : Nt
+  | S_ : Nt
+  | X_ : Nt
+  | Y_ : Nt
+  | Z_ : Nt
+  deriving DecidableEq
 
 private def a : symbol Te Nt := symbol.terminal Te.a_
 private def b : symbol Te Nt := symbol.terminal Te.b_
@@ -63,229 +65,182 @@ private def r₆ : csrule Te Nt := csrule.mk [c] Nt.C_ [] [c]
 
 
 private def my_grammar : CS_grammar Te :=
-CS_grammar.mk Nt Nt.S_ [r₁, r₂, r₃, r₃', r₃'', r₄, r₄', r₄'', r₅, r₅', r₅'', r₆]
+  CS_grammar.mk Nt Nt.S_ [r₁, r₂, r₃, r₃', r₃'', r₄, r₄', r₄'', r₅, r₅', r₅'', r₆]
+    (by intro r hr
+        simp only [List.mem_cons, List.mem_nil_iff, or_false] at hr
+        rcases hr with rfl | rfl | rfl | rfl | rfl | rfl | rfl | rfl | rfl | rfl | rfl | rfl <;>
+          simp [r₁, r₂, r₃, r₃', r₃'', r₄, r₄', r₄'', r₅, r₅', r₅'', r₆])
+
+
+-- A macro for performing one context-sensitive derivation step (with continuation).
+macro "CS_step" rule:term "," pref:term "," post:term : tactic =>
+  `(tactic| (
+    apply CS_deri_of_tran_deri
+    · refine ⟨$rule, $pref, $post, ?_, ?_, ?_⟩
+      · simp [my_grammar]
+      · rfl
+      · rfl
+  ))
 
 
 /-- generate `abc` by the grammar above -/
-example : [Te.a_, Te.b_, Te.c_] ∈ CS_language my_grammar :=
-begin
-  unfold my_grammar,
+example : [Te.a_, Te.b_, Te.c_] ∈ CS_language my_grammar := by
+  CS_step r₂, [], []
+  CS_step r₅, [a], []
+  CS_step r₅', [a], []
+  apply CS_deri_of_tran
+  · refine ⟨r₅'', [a], [], ?_, ?_, ?_⟩
+    · simp [my_grammar]
+    · rfl
+    · rfl
 
-  apply CS_deri_of_tran_deri,
-  {
-    use r₂,
-    split_ile,
-    use [[], []],
-    split;
-    refl,
-  },
-
-  apply CS_deri_of_tran_deri,
-  {
-    use r₅,
-    split_ile,
-    use [[a], []],
-    split;
-    refl,
-  },
-
-  apply CS_deri_of_tran_deri,
-  {
-    use r₅',
-    split_ile,
-    use [[a], []],
-    split;
-    refl,
-  },
-
-  apply CS_deri_of_tran,
-  {
-    use r₅'',
-    split_ile,
-    use [[a], []],
-    split;
-    refl,
-  },
-end
-
-
-private meta def CS_step (rule : pexpr) (pref post : pexpr) : tactic unit := `[
-  apply CS_deri_of_tran_deri,
-  tactic.use [rule],
-  split_ile,
-  tactic.use [pref, post],
-  split;
-  refl
-]
 
 /-- generate `aabbcc` by the grammar above -/
-example : [Te.a_, Te.a_, Te.b_, Te.b_, Te.c_, Te.c_] ∈ CS_language my_grammar :=
-begin
-  unfold my_grammar,
+example : [Te.a_, Te.a_, Te.b_, Te.b_, Te.c_, Te.c_] ∈ CS_language my_grammar := by
   -- S
-
-  CS_step ``(r₁) ``([]) ``([]),
+  CS_step r₁, [], []
   -- aSBC
-
-  CS_step ``(r₂) ``([a]) ``([B, C]),
-  -- aaRCBClet
-
-  CS_step ``(r₃)   ``([a, a, R]) ``([C]),
-  CS_step ``(r₃')  ``([a, a, R]) ``([C]),
-  CS_step ``(r₃'') ``([a, a, R]) ``([C]),
+  CS_step r₂, [a], [B, C]
+  -- aaRCBC
+  CS_step r₃,   [a, a, R], [C]
+  CS_step r₃',  [a, a, R], [C]
+  CS_step r₃'', [a, a, R], [C]
   -- aaRBCC
-
-  CS_step ``(r₄)   ``([a, a]) ``([C, C]),
-  CS_step ``(r₄')  ``([a, a]) ``([C, C]),
-  CS_step ``(r₄'') ``([a, a]) ``([C, C]),
+  CS_step r₄,   [a, a], [C, C]
+  CS_step r₄',  [a, a], [C, C]
+  CS_step r₄'', [a, a], [C, C]
   -- aabRCC
-
-  CS_step ``(r₅)   ``([a, a, b]) ``([C]),
-  CS_step ``(r₅')  ``([a, a, b]) ``([C]),
-  CS_step ``(r₅'') ``([a, a, b]) ``([C]),
+  CS_step r₅,   [a, a, b], [C]
+  CS_step r₅',  [a, a, b], [C]
+  CS_step r₅'', [a, a, b], [C]
   -- aabbcC
-
-  CS_step ``(r₆) ``([a, a, b, b]) ``([]),
+  CS_step r₆, [a, a, b, b], []
   -- aabbcc
-
-  apply CS_deri_self,
-end
+  apply CS_deri_self
 
 
-private meta def combined_steps_r₃ (pre pos : pexpr) : tactic unit := `[
-  CS_step ``(r₃)   pre pos,
-  CS_step ``(r₃')  pre pos,
-  CS_step ``(r₃'') pre pos
-]
+-- A macro for the three combined steps of rule r₃ (CB → BC).
+macro "combined_steps_r₃" pre:term "," pos:term : tactic =>
+  `(tactic| (
+    CS_step r₃,   $pre, $pos
+    CS_step r₃',  $pre, $pos
+    CS_step r₃'', $pre, $pos
+  ))
 
-private meta def combined_steps_r₄ (pre pos : pexpr) : tactic unit := `[
-  CS_step ``(r₄)   pre pos,
-  CS_step ``(r₄')  pre pos,
-  CS_step ``(r₄'') pre pos
-]
+-- A macro for the three combined steps of rule r₄ (RB → bR).
+macro "combined_steps_r₄" pre:term "," pos:term : tactic =>
+  `(tactic| (
+    CS_step r₄,   $pre, $pos
+    CS_step r₄',  $pre, $pos
+    CS_step r₄'', $pre, $pos
+  ))
 
 /-- generate `aaabbbccc` by the grammar above -/
-example : [Te.a_, Te.a_, Te.a_, Te.b_, Te.b_, Te.b_, Te.c_, Te.c_, Te.c_] ∈ CS_language my_grammar :=
-begin
+example : [Te.a_, Te.a_, Te.a_, Te.b_, Te.b_, Te.b_, Te.c_, Te.c_, Te.c_]
+    ∈ CS_language my_grammar := by
   -- S
-
-  CS_step ``(r₁) ``([]) ``([]),
+  CS_step r₁, [], []
   -- aSBC
-
-  CS_step ``(r₁) ``([a]) ``([B, C]),
+  CS_step r₁, [a], [B, C]
   -- aaSBCBC
-
-  CS_step ``(r₂) ``([a, a]) ``([B, C, B, C]),
+  CS_step r₂, [a, a], [B, C, B, C]
   -- aaaRCBCBC
-
-  combined_steps_r₃ ``([a, a, a, R]) ``([C, B, C]),
+  combined_steps_r₃ [a, a, a, R], [C, B, C]
   -- aaaRBCCBC
-
-  combined_steps_r₃ ``([a, a, a, R, B, C]) ``([C]),
+  combined_steps_r₃ [a, a, a, R, B, C], [C]
   -- aaaRBCBCC
-
-  combined_steps_r₃ ``([a, a, a, R, B]) ``([C, C]),
+  combined_steps_r₃ [a, a, a, R, B], [C, C]
   -- aaaRBBCCC
-
-  combined_steps_r₄ ``([a, a, a]) ``([B, C, C, C]),
+  combined_steps_r₄ [a, a, a], [B, C, C, C]
   -- aaabRBCCC
-
-  combined_steps_r₄ ``([a, a, a, b]) ``([C, C, C]),
+  combined_steps_r₄ [a, a, a, b], [C, C, C]
   -- aaabbRCCC
-
-  CS_step ``(r₅)   ``([a, a, a, b, b]) ``([C, C]),
-  CS_step ``(r₅')  ``([a, a, a, b, b]) ``([C, C]),
-  CS_step ``(r₅'') ``([a, a, a, b, b]) ``([C, C]),
+  CS_step r₅,   [a, a, a, b, b], [C, C]
+  CS_step r₅',  [a, a, a, b, b], [C, C]
+  CS_step r₅'', [a, a, a, b, b], [C, C]
   -- aaabbbcCC
-
-  CS_step ``(r₆) ``([a, a, a, b, b, b]) ``([C]),
+  CS_step r₆, [a, a, a, b, b, b], [C]
   -- aaabbbccC
-
-  CS_step ``(r₆) ``([a, a, a, b, b, b, c]) ``([]),
+  CS_step r₆, [a, a, a, b, b, b, c], []
   -- aaabbbccc
-
-  apply CS_deri_self,
-end
+  apply CS_deri_self
 
 
 /-- generate ` a^4 . b^4 . c^4 ` by the grammar above -/
 example : [Te.a_, Te.a_, Te.a_, Te.a_,
            Te.b_, Te.b_, Te.b_, Te.b_,
            Te.c_, Te.c_, Te.c_, Te.c_]
-    ∈ CS_language my_grammar :=
-begin
-
+    ∈ CS_language my_grammar := by
   -- .S.
-  CS_step ``(r₁) ``([]) ``([]),
+  CS_step r₁, [], []
   -- .aSBC.
 
   -- a.S.BC
-  CS_step ``(r₁) ``([a]) ``([B, C]),
+  CS_step r₁, [a], [B, C]
   -- a.aSBC.BC
 
   -- aa.S.BCBC
-  CS_step ``(r₁) ``([a, a]) ``([B, C, B, C]),
+  CS_step r₁, [a, a], [B, C, B, C]
   -- aa.aSBC.BCBC
 
   -- aaa.S.BCBCBC
-  CS_step ``(r₂) ``([a, a, a]) ``([B, C, B, C, B, C]),
+  CS_step r₂, [a, a, a], [B, C, B, C, B, C]
   -- aaa.aRC.BCBCBC
 
   -- aaaaR.CB.CBCBC
-  combined_steps_r₃ ``([a, a, a, a, R]) ``([C, B, C, B, C]),
+  combined_steps_r₃ [a, a, a, a, R], [C, B, C, B, C]
   -- aaaaR.BC.CBCBC
 
   -- aaaaRBC.CB.CBC
-  combined_steps_r₃ ``([a, a, a, a, R, B, C]) ``([C, B, C]),
+  combined_steps_r₃ [a, a, a, a, R, B, C], [C, B, C]
   -- aaaaRBC.BC.CBC
 
   -- aaaaRB.CB.CCBC
-  combined_steps_r₃ ``([a, a, a, a, R, B]) ``([C, C, B, C]),
+  combined_steps_r₃ [a, a, a, a, R, B], [C, C, B, C]
   -- aaaaRB.BC.CCBC
 
   -- aaaaRBBCC.CB.C
-  combined_steps_r₃ ``([a, a, a, a, R, B, B, C, C]) ``([C]),
+  combined_steps_r₃ [a, a, a, a, R, B, B, C, C], [C]
   -- aaaaRBBCC.BC.C
 
   -- aaaaRBBC.CB.CC
-  combined_steps_r₃ ``([a, a, a, a, R, B, B, C]) ``([C, C]),
+  combined_steps_r₃ [a, a, a, a, R, B, B, C], [C, C]
   -- aaaaRBBC.BC.CC
 
   -- aaaaRBB.CB.CCC
-  combined_steps_r₃ ``([a, a, a, a, R, B, B]) ``([C, C, C]),
+  combined_steps_r₃ [a, a, a, a, R, B, B], [C, C, C]
   -- aaaaRBB.BC.CCC
 
   -- aaaa.RB.BBCCCC
-  combined_steps_r₄ ``([a, a, a, a]) ``([B, B, C, C, C, C]),
+  combined_steps_r₄ [a, a, a, a], [B, B, C, C, C, C]
   -- aaaa.bR.BBCCCC
 
   -- aaaab.RB.BCCCC
-  combined_steps_r₄ ``([a, a, a, a, b]) ``([B, C, C, C, C]),
+  combined_steps_r₄ [a, a, a, a, b], [B, C, C, C, C]
   -- aaaab.bR.BCCCC
 
   -- aaaabb.RB.CCCC
-  combined_steps_r₄ ``([a, a, a, a, b, b]) ``([C, C, C, C]),
+  combined_steps_r₄ [a, a, a, a, b, b], [C, C, C, C]
   -- aaaabb.bR.CCCC
 
   -- aaaabbb.RC.CCC
-  CS_step ``(r₅)   ``([a, a, a, a, b, b, b]) ``([C, C, C]),
+  CS_step r₅,   [a, a, a, a, b, b, b], [C, C, C]
   -- aaaabbb.ZC.CCC
-  CS_step ``(r₅')  ``([a, a, a, a, b, b, b]) ``([C, C, C]),
+  CS_step r₅',  [a, a, a, a, b, b, b], [C, C, C]
   -- aaaabbb.Zc.CCC
-  CS_step ``(r₅'') ``([a, a, a, a, b, b, b]) ``([C, C, C]),
+  CS_step r₅'', [a, a, a, a, b, b, b], [C, C, C]
   -- aaaabbb.bc.CCC
 
   -- aaaabbbb.cC.CC
-  CS_step ``(r₆) ``([a, a, a, a, b, b, b, b]) ``([C, C]),
+  CS_step r₆, [a, a, a, a, b, b, b, b], [C, C]
   -- aaaabbbb.cc.CC
 
   -- aaaabbbbc.cC.C
-  CS_step ``(r₆) ``([a, a, a, a, b, b, b, b, c]) ``([C]),
+  CS_step r₆, [a, a, a, a, b, b, b, b, c], [C]
   -- aaaabbbbc.cc.C
 
   -- aaaabbbbcc.cC.
-  CS_step ``(r₆) ``([a, a, a, a, b, b, b, b, c, c]) ``([]),
+  CS_step r₆, [a, a, a, a, b, b, b, b, c, c], []
   -- aaaabbbbcc.cc.
 
-  apply CS_deri_self,
-end
+  apply CS_deri_self
